344. Reverse String
Solved
Easy
Topics
Companies
Hint
Write a function that reverses a string. The input string is given as an array of characters s.

You must do this by modifying the input array in-place with O(1) extra memory.

 

Example 1:

Input: s = ["h","e","l","l","o"]
Output: ["o","l","l","e","h"]
Example 2:

Input: s = ["H","a","n","n","a","h"]
Output: ["h","a","n","n","a","H"]
 

Constraints:

1 <= s.length <= 105
s[i] is a printable ascii character.

1)By Swapping:
class Solution:
    def reverseString(self, s: List[str]) -> None:
        """
        Do not return anything, modify s in-place instead.
        """
        for i in range(0,int(len(s)/2)):
            temp = s[i]
            s[i] = s[len(s)-1-i]
            s[len(s)-1-i] = temp 

2)Same Approach as above in c++:
class Solution {
public:
    void reverseString(vector<char>& s) {
        for(int i=0;i<int(s.size()/2);i++){
            swap(s[i],s[s.size()-1-i]);
        }
    }
};

3)Using Indexes:
class Solution:
    def reverseString(self, s: List[str]) -> None:
        """
        Do not return anything, modify s in-place instead.
        """
        s[:] = [s[-i-1] for i in range(len(s))]

4)Using Swap with XOR:
So swap the pairs of index (i, n-1-i). In the implementation by C, swap doesn't use extra space just by xor!
class Solution {
public:
    void reverseString(vector<char>& s) {
        for(int i=0;i<int(s.size()/2);i++){
            s[i]^=s[s.size()-1-i];// z=x^y
            s[s.size()-1-i]^=s[i];// y=z^y=(x^y)^y=x
            s[i]^=s[s.size()-1-i];// x=z^x=(x^y)^x=y
        }
    }
};

5)Two Pointer Approach:
class Solution:
    def reverseString(self, s: List[str]) -> None:
        """
        Do not return anything, modify s in-place instead.
        """
        left, right = 0, len(s) - 1
        while left < right:
            s[left], s[right] = s[right], s[left]
            left += 1
            right -= 1

6)Using Recursion:
class Solution:
    def reverseString(self, s: List[str]) -> None:
        """
        Do not return anything, modify s in-place instead.
        """
        def helper(left, right):
            if left >= right:
                return
            s[left], s[right] = s[right], s[left]
            helper(left + 1, right - 1)
        
        helper(0, len(s) - 1)

7)Most Optimized:
class Solution {
public:
    void reverseString(vector<char>& s) {
        int i = 0;
        int j = s.size() - 1;
        while (i < j) {
            char temp = s[i];  // Use char instead of int for the temporary variable
            s[i] = s[j];
            s[j] = temp;
            i++;  // Increment i to move towards the center
            j--;  // Decrement j to move towards the center
        }
    }
};